LeanScratch/Computation/RegMachine/UpdateImage.lean
@@ -1,0 +1,201 @@
+import LeanScratch.Computation.RegMachine
+
+namespace Comp
+
+def updateImageVec
+    {t : RegTree}
+    (rmapper : Fin2 n → t.toIdx)
+    (src : Vec Nat n)
+    (dst : t.toStore)
+    : t.toStore :=
+  match src with
+  | %[] => dst
+  | hd %:: tl => t.set (updateImageVec (rmapper ∘ Fin2.fs) tl dst) (rmapper .fz) hd
+
+def updateImage
+    {r t : RegTree}
+    (rmapper : r.toIdx → t.toIdx)
+    (src : r.toStore)
+    (dst : t.toStore)
+    : t.toStore :=
+  match r, src with
+  | .lf _, v => updateImageVec rmapper v dst
+  | .br _ _, ⟨lsrc, rsrc⟩ =>
+    (updateImage (rmapper ∘ Sum.inr) rsrc dst) |>
+    (updateImage (rmapper ∘ Sum.inl) lsrc ·)
+
+abbrev updateImageVec_alt
+    {t : RegTree}
+    (rmapper : Fin2 n → t.toIdx)
+    (src : Vec Nat n)
+    (dst : t.toStore)
+    : t.toStore :=
+  t.set_many dst (Fin2.instFintype2.elems.map (fun x => ⟨rmapper x, src.lookup x⟩))
+
+theorem updateImageVec_eq_alt
+    {t : RegTree}
+    {rmapper : Fin2 n → t.toIdx}
+    {src : Vec Nat n}
+    {dst : t.toStore}
+    : updateImageVec rmapper src dst =
+      updateImageVec_alt rmapper src dst :=
+  match n, src with
+  | 0, %[] => by simp [updateImageVec_alt, updateImageVec, Fin2.instFintype, RegTree.set_many]
+  | n+1, hd %:: tl => by
+    set_option pp.all true in
+    dsimp [updateImageVec, updateImageVec_alt, Fintype2.elems, RegTree.set_many, Vec.lookup]
+    rw [List.map_map]
+    congr
+    change _ = updateImageVec_alt _ _ _
+    exact updateImageVec_eq_alt
+
+/- /-- error: (kernel) deep recursion detected -/ -/
+/- #guard_msgs in -/
+/- abbrev UI_alt -/
+/-     {r t : RegTree} -/
+/-     (rmapper : r.toIdx → t.toIdx) -/
+/-     (src : r.toStore) -/
+/-     (dst : t.toStore) -/
+/-     : t.toStore := -/
+/-   t.set_many dst (RegTree.instFintype2.elems.map (fun x => ⟨rmapper x, r.lookup src x⟩)) -/
+
+theorem updateImage_eq_alt
+    {r t : RegTree}
+    {rmapper : r.toIdx → t.toIdx}
+    {src : r.toStore}
+    {dst : t.toStore}
+    : updateImage rmapper src dst =
+      t.set_many dst (RegTree.instFintype2.elems.map (fun x => ⟨rmapper x, r.lookup src x⟩)) :=
+  match r, src with
+  | .lf _, v => updateImageVec_eq_alt
+  | .br _ _, ⟨a, b⟩ => by
+    dsimp [updateImage, Fintype2.elems]
+    rw [List.map_append, List.map_map, List.map_map]
+    rw [updateImage_eq_alt, updateImage_eq_alt]
+    rw [RegTree.set_many.comp]
+    rfl
+
+theorem updateImage.comm_inj
+    {r l t : RegTree}
+    {rmapper : (r.br l).toIdx → t.toIdx}
+    {rs : r.toStore}
+    {ls : l.toStore}
+    {dst : t.toStore}
+    (hInj : Function.Injective rmapper)
+    : updateImage (rmapper ∘ Sum.inr) ls (updateImage (rmapper ∘ Sum.inl) rs dst) =
+      updateImage (rmapper ∘ Sum.inl) rs (updateImage (rmapper ∘ Sum.inr) ls dst) := by
+  rw [updateImage_eq_alt, updateImage_eq_alt, RegTree.set_many.comp, updateImage_eq_alt, updateImage_eq_alt, RegTree.set_many.comp]
+  apply RegTree.set_many.perm _ (List.perm_append_comm)
+  simp only [Function.comp_apply, List.map_append, List.map_map]
+  change List.Nodup ((List.map (rmapper ∘ Sum.inr) _) ++ (List.map (rmapper ∘ Sum.inl) _))
+  apply List.Nodup.append
+  case dj =>
+    simp only [List.Disjoint, List.mem_map, Function.comp_apply, imp_false, not_exists, not_and,
+      forall_exists_index, and_imp, forall_apply_eq_imp_iff₂]
+    exact fun _ _ _ _ h => Sum.noConfusion (hInj h)
+  all_goals apply List.Nodup.map
+  <;> (try exact Fintype2.nodup) <;> apply Function.Injective.comp hInj
+  · exact @Sum.inr.inj _ _
+  · exact @Sum.inl.inj _ _
+
+theorem updateImage.lookup.lem {r t : RegTree} {rmapper : r.toIdx → t.toIdx} {iInitStore : r.toStore}
+  {s : List r.toIdx} {outerStore : t.toStore} {reg : r.toIdx} (hInj : Function.Injective rmapper)
+  (hMem : reg ∈ s)
+  (hMem' : rmapper reg ∈ List.map rmapper s)
+  : t.lookup (t.set_many outerStore (List.map (fun x ↦ (rmapper x, r.lookup iInitStore x)) s)) (rmapper reg) =
+    r.lookup iInitStore reg := match s with
+  | [] => ((List.mem_nil_iff reg).mp hMem).elim
+  | hd :: tl => by
+    dsimp [RegTree.set_many]
+    by_cases h : reg = hd
+    · subst h
+      rw [RegTree.lookup_set_eq]
+    · rw [RegTree.lookup_set_ne (h $ hInj ·.symm)]
+      apply updateImage.lookup.lem hInj (List.mem_of_ne_of_mem h hMem)
+      simp_all
+
+theorem updateImage.lookup
+    {r t : RegTree}
+    {rmapper : r.toIdx → t.toIdx}
+    {iInitStore outerStore}
+    {reg : r.toIdx}
+    (hInj : Function.Injective rmapper)
+    : t.lookup (updateImage rmapper iInitStore outerStore) (rmapper reg) =
+      r.lookup iInitStore reg := by
+  rw [updateImage_eq_alt]
+  let regMem : reg ∈ _ := Fintype2.complete reg
+  let rMapperReg : rmapper reg ∈ List.map rmapper _ := List.mem_map_of_mem rmapper regMem
+  exact updateImage.lookup.lem hInj regMem rMapperReg
+
+theorem updateImage.set
+    {r t : RegTree}
+    {rmapper : r.toIdx → t.toIdx}
+    {iInitStore outerStore}
+    {reg : r.toIdx}
+    (hInj : Function.Injective rmapper)
+    : t.set (updateImage rmapper iInitStore outerStore) (rmapper reg) v =
+      updateImage rmapper (r.set iInitStore reg v) outerStore := by
+  ext z
+  by_cases h : z = rmapper reg
+  · subst h
+    rw [updateImage.lookup hInj]
+    simp
+  · have hSymm : rmapper reg ≠ z := h ∘ Eq.symm
+    rw [RegTree.lookup_set_ne hSymm]
+    by_cases h : ∃ k, z = rmapper k
+    · rcases h with ⟨z, rfl⟩
+      rw [updateImage.lookup hInj, updateImage.lookup hInj]
+      rw [RegTree.lookup_set_ne]
+      exact fun a => h $ a.rec rfl
+    · rw [not_exists] at h
+      rw [updateImage_eq_alt, updateImage_eq_alt]
+      rw [RegTree.lookup_set_many_none, RegTree.lookup_set_many_none]
+      <;> simp only [Nat.succ_eq_add_one, List.map_map, List.mem_map, Fintype2.complete,
+        Function.comp_apply, true_and, not_exists]
+      <;> exact fun z eq => h z eq.symm
+
+theorem updateImage.inc_slide
+    {r t : RegTree}
+    {rmapper : r.toIdx → t.toIdx}
+    {iInitStore outerStore}
+    {reg : r.toIdx}
+    (hInj : Function.Injective rmapper)
+    : RegMachine.inc (rmapper reg) (updateImage rmapper iInitStore outerStore) =
+      updateImage rmapper (RegMachine.inc reg iInitStore) outerStore := by
+  rw [RegMachine.inc.eq_set,
+      RegMachine.inc.eq_set,
+      updateImage.lookup hInj,
+      updateImage.set hInj]
+
+theorem updateImage.dec_slide
+    {r t : RegTree}
+    {rmapper : r.toIdx → t.toIdx}
+    {iInitStore outerStore}
+    {reg : r.toIdx}
+    (hInj : Function.Injective rmapper)
+    : RegMachine.dec (rmapper reg) (updateImage rmapper iInitStore outerStore) =
+      (RegMachine.dec reg iInitStore).map (updateImage rmapper · outerStore)
+      := by
+  by_cases h : ∃ z, RegMachine.dec reg iInitStore = some z
+  · -- Begin intense bit of proof
+    have ⟨k, hKEq⟩ := Nat.exists_eq_succ_of_ne_zero
+        $ (not_congr RegMachine.dec_none_iff_lookup_z).mp
+        $ Option.ne_none_iff_exists'.mpr h
+    have : t.lookup (updateImage rmapper iInitStore outerStore) (rmapper reg) = k.succ :=
+      Eq.trans (updateImage.lookup hInj) hKEq
+    have ⟨w', hBigEqSome⟩ := Option.ne_none_iff_exists'.mp
+        $ (not_congr RegMachine.dec_none_iff_lookup_z).mpr
+        (Nat.noConfusion $ Eq.trans ·.symm this)
+    rcases h with ⟨w, hEqSome⟩
+    -- end intense bit of proof
+    rw [hEqSome,    RegMachine.dec.eq_set hEqSome,
+        hBigEqSome, RegMachine.dec.eq_set hBigEqSome]
+    clear *-hInj
+    apply (Option.some.injEq _ _).mpr
+    dsimp
+    rw [updateImage.lookup hInj, updateImage.set hInj]
+  · simp only [← Option.ne_none_iff_exists', ne_eq, not_not] at h
+    have : t.lookup (updateImage rmapper iInitStore outerStore) (rmapper reg) = 0 :=
+      Eq.trans (updateImage.lookup hInj) (RegMachine.dec_none_iff_lookup_z.mp h)
+    rw [RegMachine.dec_none_iff_lookup_z.mpr this, h]
+    rfl
